Generalize void elimination.

theories/void.v
@@ -2,17 +2,17 @@ From mathcomp Require Import ssreflect ssrfun eqtype choice fintype.
 
 Notation void := Empty_set.
 
-Definition unit_of_void (x : void) : unit := tt.
-Definition void_of_unit (x : unit) : option void := None.
+Definition of_void T (x : void) : T := match x with end.
+Definition to_void T (x : T) : option void := None.
 
-Lemma unit_of_voidK : pcancel unit_of_void void_of_unit.
+Lemma of_voidK T : pcancel (@of_void T) (@to_void T).
 Proof. by case. Qed.
 
-Definition void_eqMixin := PcanEqMixin unit_of_voidK.
+Definition void_eqMixin := PcanEqMixin (of_voidK unit).
 Canonical void_eqType := Eval hnf in EqType void void_eqMixin.
-Definition void_choiceMixin := PcanChoiceMixin unit_of_voidK.
+Definition void_choiceMixin := PcanChoiceMixin (of_voidK unit).
 Canonical void_choiceType := Eval hnf in ChoiceType void void_choiceMixin.
-Definition void_countMixin := PcanCountMixin unit_of_voidK.
+Definition void_countMixin := PcanCountMixin (of_voidK unit).
 Canonical void_countType := Eval hnf in CountType void void_countMixin.
-Definition void_finMixin := PcanFinMixin unit_of_voidK.
+Definition void_finMixin := PcanFinMixin (of_voidK unit).
 Canonical void_finType := Eval hnf in FinType void void_finMixin.
